[repdb] wip on resources.

ml_sources/examples/reliable_communication/lib/repdb/repdb_code.ml
@@ -100,7 +100,7 @@ let start_follower_processing_clients (ser[@metavar]) addr db mon =
   run_server (rep_f2c_ser ser) req_c2f_ser addr mon
     (client_request_handler_at_follower db)
 
-let sync_loop db log mon reqf : unit =
+let sync_loop db log mon reqf () : unit =
   let rec aux () =
     let i = log_next log in
     let rep = reqf i in
@@ -115,7 +115,7 @@ let sync_loop db log mon reqf : unit =
 
 let sync_with_server (ser[@metavar]) l_addr f2l_addr db log mon : unit =
   let reqf = init_client_proxy req_f2l_ser (rep_l2f_ser ser) f2l_addr l_addr in
-  sync_loop db log mon reqf
+  fork (sync_loop db log mon reqf) ()
 
 (** Initialization of the follower. *)
 let init_follower (ser[@metavar]) l_addr f2l_addr f_addr  =
