aneris/examples/reliable_communication/lib/repdb/spec/ras.v
@@ -1,42 +1,36 @@
 From iris.algebra Require Import auth gmap excl excl_auth.
-From aneris.algebra Require Import monotone.
+From iris.algebra.lib Require Import mono_list.
+From aneris.lib Require Import gen_heap_light.
 From aneris.aneris_lang.lib Require Import lock_proof.
 From aneris.examples.reliable_communication.lib.repdb.spec
      Require Import db_params time events resources.
 
 
-Class DBG `{!DB_time, !DB_events} Σ :=
-  {
-    DBG_Global_mem_excl :>
-      inG Σ (authUR (gmapUR Key (prodR fracR (agreeR (optionO (leibnizO we))))));
-    DBG_Global_history_mono :>
-      inG Σ (authUR (monotoneUR (@prefix (leibnizO we))));
-    DBG_Local_history_mono :>
-      inG Σ (gmapUR socket_address (agreeR gnameO));
-    DBG_lockG :>
-      lockG Σ;
-    DBG_followers_gname : gname;
+Class DBG `{!DB_time} Σ :=
+  { DBG_Global_mem :> inG Σ (authR (gen_heapUR Key (option we)));
+    DBG_Global_history_mono :> inG Σ (mono_listUR (leibnizO we));
+    DBG_Known_replog :> inG Σ (authR (gmapUR socket_address (agreeR gnameO)));
+    DBG_free_replogG :> inG Σ (gset_disjUR socket_address);
+    DBG_lockG :> lockG Σ;
+    DBG_known_replog_name : gname;
+    DBG_free_replog_set_name : gname;
+  }.
 
-}.
+Class DBPreG `{!DB_time} Σ :=
+  { DB_preG_Global_mem :> inG Σ (authR (gen_heapUR Key (option we)));
+    DB_preG_Global_history_mono :> inG Σ (mono_listUR (leibnizO we));
+    DB_preG_Known_replog :>
+      inG Σ (authR (gmapUR socket_address (agreeR gnameO)));
+    DB_preG_free_replogG :> inG Σ (gset_disjUR socket_address);
+    DB_preG_lockG :> lockG Σ;
+  }.
 
-Class DBPreG `{!DB_time, !DB_events} Σ :=
-  {
-    DBG_preGlobal_mem_excl :>
-      inG Σ (authUR (gmapUR Key (prodR fracR (agreeR (optionO (leibnizO we))))));
-    DBG_preGlobal_history_mono :>
-      inG Σ (authUR (monotoneUR (@prefix (leibnizO we))));
-    DBG_preLocal_history_mono :>
-      inG Σ (gmapUR socket_address (agreeR gnameO));
-    DBG_prelockG :>
-      lockG Σ;
-}.
-
-
-Definition DBΣ `{!DB_time, !DB_events} : gFunctors :=
-  #[GFunctor (authUR (gmapUR Key (prodR fracR (agreeR (optionO (leibnizO we))))));
-    GFunctor (authUR (monotoneUR (@prefix (leibnizO we))));
-    GFunctor (gmapUR socket_address (agreeR gnameO));
+Definition DBΣ `{!DB_time} : gFunctors :=
+  #[GFunctor (authR (gen_heapUR Key (option we)));
+    GFunctor (mono_listUR (leibnizO we));
+    GFunctor (authR (gmapUR socket_address (agreeR gnameO)));
+    GFunctor (gset_disjUR socket_address);
     lockΣ].
 
-Instance subG_DB_preGΣ `{!DB_time, !DB_events, !lockG Σ} : subG DBΣ Σ → DBPreG Σ.
+Instance subG_DB_preGΣ `{!DB_time, !lockG Σ} : subG DBΣ Σ → DBPreG Σ.
 Proof. solve_inG. Qed.
