aneris/examples/reliable_communication/lib/repdb/spec/time.v
@@ -4,40 +4,29 @@ From stdpp Require Import gmap.
 
 Section Time.
 
+
   Class DB_time := {
     Time : Type;
-    TM_lt' : relation Time;
-    TM_lt := strict TM_lt';
-    TM_lt_TO :> TotalOrder (TM_lt);
+    TM_lt : relation Time;
+    TM_lt_TO :> StrictOrder TM_lt;
+    TM_lt_tricho : ∀ m n : Time, TM_lt m n ∨ m = n ∨ TM_lt n m;
     TM_EqDecision :> EqDecision Time;
+    TM_Countable :> Countable Time;
+    (* TM_max : Time → Time → Time. TODO *)
    }.
 
-  Class Timed {dbt: DB_time} (T : Type) := time : T → Time.
+  (* Class Timed {dbt: DB_time} (T : Type) := time : T → Time. *)
 
-  Notation "t1 '<ₜ' t2" :=
-    (TM_lt (time t1) (time t2)) (at level 70, no associativity).
-  Notation "t1 '≤ₜ' t2" :=
-    (TM_lt (time t1) (time t2) ∨ (time t1 = time t2)) (at level 70, no associativity).
-  Notation "t1 '=ₜ' t2" :=
-    (time t1 = time t2) (at level 70, no associativity).
-
-  Definition IsMaximum {T : Type} `{!DB_time} `{!EqDecision T}
-             `{!Countable T} `{!Timed T} (X : gset T) (mx : T) :=
-    mx ∈ X ∧ ∀ t, t ∈ X → (¬ t = mx) → t <ₜ mx.
-
-  Class Maximals_Computing `{!DB_time} :=
-    {
-      Maximum : ∀ {T : Type} `{!EqDecision T} `{!Countable T}
-           `{!Timed T} (X : gset T), option T;
-      Maximum_correct : ∀ {T : Type} `{!EqDecision T} `{!Countable T}
-           `{!Timed T} (X : gset T),
-          (∀ x y, x ∈ X → y ∈ X → x =ₜ y → x = y) →
-          (∀ x, Maximum X = Some x ↔ IsMaximum X x);
-    }.
-
+  (* Notation "s '<ₜ' t" := *)
+  (*   (TM_lt (time s) (time t)) (at level 70, no associativity). *)
+  (* Notation "t1 '≤ₜ' t2" := *)
+  (*   (TM_lt (time t1) (time t2) ∨ (time t1 = time t2)) *)
+  (*     (at level 70, no associativity). *)
+  (* Notation "t1 '=ₜ' t2" := *)
+  (*   (time t1 = time t2) (at level 70, no associativity). *)
   End Time.
 
-
+(*
 Notation "s '<ₜ@{' d '}' t" :=
   (TM_lt (@time d _ _ s) (@time d _ _ t))
     (at level 70, no associativity, format "s  '<ₜ@{' d '}'  t").
@@ -47,10 +36,11 @@ Notation "s '≤ₜ@{' d '}' t" :=
 Notation "s '=ₜ@{' d '}' t" :=
   ((@time d _ _ s) = (@time d _ _ t))
     (at level 70, no associativity, format "s  '=ₜ@{' d '}'  t").
+*)
 
-Notation "s '<ₜ' t" :=
-  (TM_lt (time s) (time t)) (at level 70, no associativity).
-Notation "s '≤ₜ' t" :=
-  (TM_lt (time s) (time t) ∨ (time s = time t)) (at level 70, no associativity).
-Notation "s '=ₜ' t" :=
-  (time s = time t) (at level 70, no associativity).
+(* Notation "s '<ₜ' t" := *)
+(*   (TM_lt (time s) (time t)) (at level 70, no associativity). *)
+(* Notation "s '≤ₜ' t" := *)
+(*   (TM_lt (time s) (time t) ∨ (time s = time t)) (at level 70, no associativity). *)
+(* Notation "s '=ₜ' t" := *)
+(*   (time s = time t) (at level 70, no associativity). *)
