aneris/examples/reliable_communication/lib/repdb/resources/resources.v
@@ -1,0 +1,282 @@
+From iris.algebra Require Import agree auth excl gmap dfrac.
+From iris.algebra.lib Require Import mono_list.
+From iris.base_logic Require Import invariants.
+From iris.bi.lib Require Import fractional.
+From iris.proofmode Require Import tactics.
+From aneris.lib Require Import gen_heap_light.
+From aneris.aneris_lang Require Import lang resources inject.
+From aneris.aneris_lang.lib Require Import lock_proof.
+From aneris.examples.reliable_communication.lib.repdb.spec
+     Require Import db_params time events.
+From aneris.examples.reliable_communication.lib.repdb.resources
+     Require Import time.
+Import gen_heap_light.
+
+
+Instance: Inhabited (@we int_time) := populate (Build_we "" #() inhabitant).
+
+Global Program Instance Inject_write_event : Inject we val :=
+  {| inject a := $(a.(we_key), a.(we_val), a.(we_time))
+  |}.
+Next Obligation.
+  intros w1 w2 Heq.
+  inversion Heq as [[Hk Hv Ht]].
+  assert (we_time w1 = we_time w2) as Ht'.
+  { by apply (inj (R := eq)) in Ht; [ | apply _]. }
+  destruct w1, w2; simpl in *.
+  by apply Z_of_nat_inj in Ht; subst.
+Qed.
+
+Definition write_event := @we int_time.
+Definition write_eventO := leibnizO write_event.
+Definition wrlog := list write_eventO.
+
+(* -------------------------------------------------------------------------- *)
+Class IDBG Σ :=
+  { IDBG_Global_mem :>
+      inG Σ (authR (gen_heapUR Key (option write_event)));
+    IDBG_Global_history_mono :>
+      inG Σ (mono_listUR write_eventO);
+    IDBG_Known_replog :>
+      inG Σ (authR (gmapUR socket_address (agreeR gnameO)));
+    IDBG_free_replogG :>
+      inG Σ (gset_disjUR socket_address);
+    IDBG_lockG :> lockG Σ;
+    IDBG_known_replog_name : gname;
+    IDBG_free_replog_set_name : gname;
+  }.
+
+Section ValidStates.
+  Context `{!anerisG Mdl Σ, !DB_params}.
+
+  (** Validity. *)
+  Definition mem_dom (M : gmap Key (option write_event)) := DB_keys = dom M.
+
+  Definition mem_we_key (M : gmap Key (option write_event)) :=
+    ∀ k (we : write_event), k ∈ dom M →
+                            M !! k = Some (Some we) → we.(we_key) = k.
+
+  Definition mem_log_coh (L : wrlog) (M : gmap Key (option write_event)) :=
+    ∀ k, k ∈ dom M → M !! k = Some (at_key k L).
+
+  Definition allocated_in_mem (L : wrlog) (M : gmap Key (option write_event)) :=
+    ∀ l k wel, l ≤ₚ L → at_key k l = Some wel →
+               ∃ weL, M !! k = Some (Some weL) ∧ wel ≤ₜ weL.
+
+  Definition log_events (L : wrlog) :=
+    ∀ i, 0 <= i → i < List.length L →
+         ∃ we, List.nth_error L i = Some we ∧ i = we.(we_time).
+
+  Record valid_state (L : wrlog) (M : gmap Key (option write_event)) : Prop :=
+    {
+      DB_GSTV_mem_dom : mem_dom M;
+      DB_GSTV_mem_we_key : mem_we_key M;
+      DB_GSTV_mem_log_coh : mem_log_coh L M;
+      DB_GSTV_mem_allocated_in_mem : allocated_in_mem L M;
+      DB_GSTV_log_events L : log_events L;
+    }.
+
+End ValidStates.
+
+Section Resources.
+  Context `{!anerisG Mdl Σ, !DB_params, !IDBG Σ}.
+  Context (γL γM : gname).
+
+  (** Abstract global memory. *)
+
+  Definition own_mem_user (k : Key) (q: Qp) (a : option write_event) :=
+    lmapsto γM k q a.
+
+  Definition own_mem_sys M := gen_heap_light_ctx γM M.
+
+  (** Properties of points-to connective *)
+  Lemma OwnMemKey_timeless_holds k q v : Timeless (own_mem_user k q v).
+  Proof. Admitted.
+  Lemma OwnMemKey_exclusive_holds k q v v' :
+    own_mem_user k 1 v ⊢ own_mem_user k q v' -∗ False.
+  Proof. Admitted.
+
+  Lemma OwnMemKey_fractioal_holds k v : Fractional (λ q, own_mem_user k q v).
+  Proof. Admitted.
+
+  Lemma OwnMemKey_as_fractioal_holds k q v :
+    AsFractional (own_mem_user k q v) (λ q, own_mem_user k q v) q.
+  Proof. Admitted.
+
+  Lemma OwnMemKey_combine_holds k q q' v v' :
+    own_mem_user k q v ∗ own_mem_user k q' v ⊢
+    own_mem_user k (q + q') v ∗ ⌜v = v'⌝.
+  Proof. Admitted.
+
+  Lemma OwnMemKey_split_holds k q1 q2 v :
+    own_mem_user k (q1 + q2) v ⊢ own_mem_user k q1 v ∗ own_mem_user k q2 v.
+  Proof. Admitted.
+
+  (** Log resources. *)
+
+  (** Owned by global invariant of the system. *)
+  Definition own_log_global (γ : gname) (l : wrlog) : iProp Σ :=
+    own γ (●ML{ DfracOwn (1/2) } l).
+
+  (** Owned by the lock invariant of a replica *)
+  Definition own_log_local (γ : gname) (l : wrlog) : iProp Σ :=
+    own γ (●ML{ DfracOwn (1/2) } l).
+
+  (** Duplicable observation describing the prefix of a log. *)
+  Definition own_log_obs (γ : gname) (l : wrlog) : iProp Σ :=
+    own γ (◯ML l).
+
+  (** Resources about free/known replicated logs. *)
+
+  (** Ownership to create a new replicated log. *)
+  Definition free_replog_token (sa : socket_address) : iProp Σ :=
+    own IDBG_free_replog_set_name (GSet {[sa]}).
+
+  (** Ownership for a replicated log known by the system. *)
+  Definition known_replog_token (sa : socket_address) (γ : gname) : iProp Σ :=
+    own IDBG_known_replog_name (◯ {[ sa := to_agree γ ]}).
+
+  (** Ownership of all replicated logs known by the system. *)
+  Definition known_replog_tokens (N : gmap socket_address gname)  : iProp Σ :=
+    own IDBG_free_replog_set_name (GSet (dom N)) ∗
+      own IDBG_known_replog_name (● (to_agree <$> N : gmap _ _ )).
+
+  (** Principal log *)
+
+  Definition own_logL_global L : iProp Σ := own γL (●ML{ DfracOwn (1/2) } L).
+
+  Definition own_logL_local L : iProp Σ := own γL (●ML{ DfracOwn (1/2) } L).
+
+  Definition own_logL_obs L : iProp Σ := own γL (◯ML L).
+
+  (** Replicated logs. *)
+
+  Definition own_replog_global γ sa l : iProp Σ :=
+    known_replog_token sa γ ∗ own_logL_obs l ∗ own_log_global γ l.
+
+  Definition own_replog_local sa l : iProp Σ :=
+    ∃ γ, known_replog_token sa γ ∗ own_logL_obs l ∗ own_log_local γ l.
+
+  Definition own_replog_obs sa l : iProp Σ :=
+    ∃ γ, known_replog_token sa γ ∗ own_logL_obs l.
+
+  (** General Obs predicate : socket_address → wrlog → iProp Σ. *)
+  Definition own_obs sa l : iProp Σ :=
+    (⌜sa = DB_addr⌝ ∗ own_logL_obs l) ∨ own_replog_obs sa l.
+
+  Lemma Obs_timeless_holds a h : Timeless (own_obs a h).
+  Proof. apply _. Qed.
+
+  Lemma Obs_persistent_holds a h : Persistent (own_obs a h).
+  Proof. apply _. Qed.
+
+  (** Definition of the global invariant. *)
+  Definition global_inv_def : iProp Σ :=
+    ∃ (L : wrlog)
+      (M : gmap Key (option write_event))
+      (N: gmap socket_address gname),
+      ⌜DB_keys = dom M⌝ ∗
+      own_mem_sys M ∗
+      own_logL_global L ∗
+      known_replog_tokens N ∗
+      ([∗ map] sa ↦ γ ∈ N, ∃ l, own_replog_global γ sa l) ∗
+      ⌜valid_state L M⌝.
+
+  Definition Global_Inv := inv DB_InvName global_inv_def.
+
+  Lemma Global_InvPersistent : Persistent Global_Inv.
+  Proof. apply _. Qed.
+
+  Lemma OwnMemKey_key_holds k q we E :
+    nclose DB_InvName ⊆ E →
+    Global_Inv ⊢
+    own_mem_user k q (Some we) ={E}=∗
+    own_mem_user k q (Some we) ∗ ⌜we_key we = k⌝.
+  Proof. Admitted.
+
+  Lemma Obs_compare_holds a a' h h' E :
+    nclose DB_InvName ⊆ E →
+    Global_Inv ⊢ own_obs a h -∗ own_obs a' h' ={E}=∗
+    ⌜h ≤ₚ h'⌝ ∨ ⌜h' ≤ₚ h⌝.
+  Proof. Admitted.
+
+  Lemma Obs_exists_at_leader_holds a1 h1 E:
+    ↑DB_InvName ⊆ E → Global_Inv ⊢
+    own_obs a1 h1 ={E}=∗ ∃ h2, own_obs DB_addr h2 ∗ ⌜h1 ≤ₚ h2⌝.
+  Proof. Admitted.
+
+  Lemma Obs_get_smaller_holds a h h' E :
+    nclose DB_InvName ⊆ E →
+    h ≤ₚ h' →
+    own_obs a h' ={E}=∗ own_obs a h.
+  Proof. Admitted.
+
+  Lemma Obs_snoc_time_holds a h1 e1 h2 E :
+    nclose DB_InvName ⊆ E →
+    own_obs a (h1 ++ [e1] ++ h2) ={E}=∗
+    ⌜∀ e0, e0 ∈ h1 → e0 <ₜ e1⌝ ∧ ⌜∀ e2, e2 ∈ h2 → e1 <ₜ e2⌝.
+  Proof. Admitted.
+
+  Lemma Obs_ext_we_holds a a' h h' E :
+    nclose DB_InvName ⊆ E →
+    Global_Inv ⊢ own_obs a h -∗ own_obs a' h' ={E}=∗
+    ⌜∀ e e', e ∈ h → e' ∈ h' → e =ₜ e' → e = e'⌝.
+  Proof. Admitted.
+
+  Lemma Obs_ext_hist_holds a1 a2 h1 h2 k E :
+    nclose DB_InvName ⊆ E →
+    at_key k h1 = at_key k h2 →
+    Global_Inv ⊢ own_obs a1 h1 -∗ own_obs a2 h2 ={E}=∗
+    ⌜hist_at_key k h1 = hist_at_key k h2⌝.
+  Proof. Admitted.
+
+  Lemma OwnMemKey_some_obs_we_holds k q we E :
+    nclose DB_InvName ⊆ E →
+    Global_Inv ⊢
+    own_mem_user k q (Some we) ={E}=∗
+    own_mem_user k q (Some we) ∗
+      ∃ h, own_obs DB_addr h ∗ ⌜at_key k h = Some we⌝.
+  Proof. Admitted.
+
+  Lemma OwnMemKey_obs_frame_prefix_holds a k q h h' E :
+    nclose DB_InvName ⊆ E →
+    h ≤ₚ h' →
+    Global_Inv ⊢
+    own_mem_user k q (at_key k h) ∗ own_obs a h' ={E}=∗
+    own_mem_user k q (at_key k h) ∗ ⌜at_key k h = at_key k h'⌝.
+  Proof. Admitted.
+
+  Lemma OwnMemKey_obs_frame_prefix_some_holds a k q h h' we E :
+    nclose DB_InvName ⊆ E →
+    h ≤ₚ h' →
+    at_key k h = Some we →
+    Global_Inv ⊢
+    own_mem_user k q (Some we) ∗ own_obs a h' ={E}=∗
+    own_mem_user k q (Some we) ∗ ⌜at_key k h' = Some we⌝.
+  Proof. Admitted.
+
+  Lemma OwnMemKey_some_obs_frame_holds a k q we h hf E :
+    nclose DB_InvName ⊆ E →
+    Global_Inv ⊢
+    own_mem_user k q (Some we) ∗ own_obs a (h ++ [we] ++ hf) ={E}=∗
+    own_mem_user k q (Some we) ∗ ⌜at_key k hf = None⌝.
+  Proof. Admitted.
+
+  Lemma OwnMemKey_none_obs_holds a k q h E :
+    nclose DB_InvName ⊆ E →
+    Global_Inv ⊢
+      own_mem_user k q None ∗ own_obs a h ={E}=∗
+      own_mem_user k q None ∗ ⌜hist_at_key k h = []⌝.
+  Proof. Admitted.
+
+  Lemma OwnMemKey_allocated_holds k q h0 h1 we0 E :
+    nclose DB_InvName ⊆ E →
+    h0 ≤ₚ h1 →
+    at_key k h0 = Some we0 →
+    Global_Inv ⊢
+    own_mem_user k q (at_key k h1) ={E}=∗
+    ∃ we1, own_mem_user k q (at_key k h1) ∗
+             ⌜at_key k h1 = Some we1⌝ ∗ ⌜we0 ≤ₜ we1⌝.
+  Proof. Admitted.
+
+End Resources.
