aneris/examples/reliable_communication/lib/repdb/resources/time.v
@@ -1,0 +1,9 @@
+From aneris.aneris_lang Require Import lang.
+From aneris.examples.reliable_communication.lib.repdb.spec
+     Require Import time.
+
+
+Global Instance int_time : DB_time :=
+  {| Time := nat;
+    TM_lt := Nat.lt;
+    TM_lt_tricho := PeanoNat.Nat.lt_trichotomy |}.
