aneris/examples/reliable_communication/lib/repdb/spec/utils.v
@@ -8,7 +8,7 @@ Section with_Σ.
   (* TODO: maybe add frame after [we1] here *)
   Lemma OwnMemKey_Obs_extend a E h k we1 we2 :
     nclose DB_InvName ⊆ E →
-    WE_key we1 = WE_key we2 →
+    we_key we1 = we_key we2 →
     we1 ≠ we2 →
     GlobalInv -∗
     Obs a (h ++ [we1]) -∗
@@ -17,17 +17,17 @@ Section with_Σ.
     ∃ hf, Obs DB_addr (h ++ [we1] ++ hf ++ [we2]).
   Proof.
     iIntros (HE Heq Hneq) "#HGinv #Hobs Hk".
-    iMod (OwnMemKey_key with "Hk") as "[Hk %Hkey]"; [solve_ndisj|].
+    iMod (OwnMemKey_key with "[$HGinv][$Hk]") as "[Hk %Hkey]"; [solve_ndisj|].
     iMod (OwnMemKey_some_obs_we with "[$HGinv][$Hk]") as "[Hk (%h' & #Hobs' & %Hatkey)]"; [solve_ndisj|].
     iMod (Obs_compare with "HGinv Hobs Hobs'") as %Hle; [solve_ndisj|].
     destruct Hle as [Hle | Hle]; last first.
     { (* Solve contradiction *)
-      iMod (OwnMemKey_obs_frame_prefix_some with "[$Hk $Hobs]")
+      iMod (OwnMemKey_obs_frame_prefix_some with "[$HGinv][$Hk $Hobs]")
         as "[Hk %Hatkey']"; [solve_ndisj|done..|].
       rewrite at_key_snoc_some in Hatkey'; naive_solver. }
     assert (Some we2 = at_key k h') as ->.
     { by rewrite Hatkey. }
-    iMod (OwnMemKey_allocated with "Hk") as "(%we' & Hk & %Hatkey' & %Hle')";
+    iMod (OwnMemKey_allocated with "[$HGinv][$Hk]") as "(%we' & Hk & %Hatkey' & %Hle')";
       [solve_ndisj|done|apply at_key_snoc_some; naive_solver|].
     assert (we' = we2) as -> by naive_solver. clear Hatkey'.
     iFrame "Hk".
